feat: add Foldable methods

Sat/Lib/Foldable.lean
@@ -1,9 +1,14 @@
 
 import Sat.Lib.Array.Basic
+import Sat.Lib.List.Basic
 import Sat.Lib.Monoid
 
 class Foldable (F : Type u → Type v) where
   foldl {α β : Type u} (f : β → α → β) (x₀ : β) (t : F α) : β
+  toList {α} (x : F α) : List α := foldl (flip (.::.)) [] x |>.reverse
+  toArray {α} (x : F α) : Array α := toList x |>.toArray
+  length {α} (x : F α) : Nat :=
+    ULift.down <| foldl (λ n _ => ⟨n.1.succ⟩) ⟨0⟩ x
 
 namespace Foldable
 
@@ -18,13 +23,71 @@ end Foldable
 open One
 
 open Foldable
+
+macro "prove_length_toList" sim:ident α:ident x:ident : tactic =>
+  `(tactic|
+       -- intros α x;
+       suffices H : ((foldl (flip (.::.)) [] x).length =
+                 ULift.down (foldl (β := ULift Nat)
+                            (λ ⟨n⟩ _ => ⟨n.succ⟩) ⟨0⟩ x))
+                by {trans <;> try assumption};
+       let R :=
+         λ (x : List α) (y : ULift Nat) => x.length = y.down;
+       apply sim (SIM := R)
+       . apply Reflexive.refl
+       . simp [flip]; auto)
+
+macro "prove_foldl_toList" sim:term : tactic =>
+  `(tactic|
+       intros α β f x₀ x;
+       suffices H : ((foldl (flip (.::.)) [] x).foldl f x₀ x =
+                 foldl f x₀ x)
+                by {trans <;> try assumption};
+       let R :=
+         λ (x : List α) (y : β) => x.reverse.foldl f x₀ x = y;
+       apply sim (SIM := R)
+       . apply Reflexive.refl
+       . simp [flip]; auto)
+
 class LawfulFoldable (F : Type u → Type v) [Foldable F] where
   foldl_sim {α β γ : Type u} {f : β → α → β} {g : γ → α → γ} {SIM : β → γ → Prop} {x₀ y₀} (t : F α) :
     SIM x₀ y₀ →
     (∀ a x y, SIM x y → SIM (f x a) (g y a)) →
     SIM (foldl f x₀ t) (foldl g y₀ t)
+  toArray_toList {α} (x : F α) : (toList x).toArray = toArray x
+    -- by apply Reflexive.refl
+  length_toList {α} (x : F α) : (toList x).length = length x
+ -- :=
+ --    -- let H := @foldl_sim
+ --    -- by prove_length_toList H α x
+ --       have H' : ∀ xs n, List.length xs = n → List.length xs.reverse = n := sorry
+ --       suffices H : ((foldl (flip (.::.)) [] x).length =
+ --                 ULift.down (foldl (β := ULift Nat)
+ --                            (λ ⟨n⟩ _ => ⟨n.succ⟩) ⟨0⟩ x))
+ --                by apply H' _ _ H
+ --       let R :=
+ --         λ (x : List α) (y : ULift Nat) => x.length = y.down;
+ --       by apply foldl_sim (SIM := R)
+ --          . apply Reflexive.refl
+ --          . simp [flip]; auto
+  foldl_toList {α β} (f : β → α → β) (x₀ : β) (x : F α) :
+    (toList x).foldl f x₀ = foldl f x₀ x
+ -- :=
+ --    -- let H := @foldl_sim
+ --    -- by prove_foldl_toList H
+ --       suffices H : ((foldl (flip (.::.)) [] x).reverse.foldl f x₀ =
+ --                 foldl f x₀ x)
+ --                by {trans <;> try assumption}
+ --       let R :=
+ --         λ (l : List α) (y : β) => l.reverse.foldl f x₀ = y;
+ --       by
+ --          apply foldl_sim (SIM := R) x
+ --       -- apply sim (SIM := R)
+ --          . apply Reflexive.refl
+ --          focus simp [flip]
 
 namespace LawfulFoldable
+attribute [simp] length_toList toArray_toList
 
 variable {F} [Foldable F] [LawfulFoldable F]
 
@@ -43,17 +106,60 @@ variable (f : MonoidHom α β)
 
 variable {γ : Type u}
 
-def foldMap_hom (g₀ : γ → α) (x : F γ) :
+theorem foldMap_hom (g₀ : γ → α) (x : F γ) :
   f (foldMap g₀ x) = foldMap (f ∘ g₀) x := by
 apply foldl_hom <;> intros <;> simp
+
+@[simp]
+theorem toList_toArray {α} (x : F α) : (toArray x).toList = toList x := by
+rw [← toArray_toList, Array.toList_toArray]
+
+@[simp]
+theorem size_toArray {α} (x : F α) : (toArray x).size = length x := by
+rw [← toArray_toList]; simp [-toArray_toList]
+
+theorem foldl_toArray {α β} (f : β → α → β) (x₀ : β) (x : F α) :
+    (toArray x).foldl f x₀ = foldl f x₀ x := by
+rw [← toArray_toList]; simp [-toArray_toList]
+rw [Array.foldl_toArray, foldl_toList]
+rw [length_toList]
+
+theorem toList_eq (x : F α) :
+  toList x = (foldl (flip (.::.)) [] x).reverse := by
+rw [← foldl_toList, List.foldl_eq_self]
+
+theorem toArray_eq (x : F α) :
+  toArray x = (foldl Array.push #[] x) := by
+rw [← toArray_toList, ← foldl_toList]
+generalize toList x = xs; clear x
+simp only [List.toArray]
+simp [List.toArrayAux, Array.mkEmpty_eq_mkEmpty 0]
+generalize (Array.mkEmpty 0) = ar
+induction xs generalizing ar
+ <;> simp [List.toArrayAux, List.foldl, *]
+
+theorem length_eq (x : F α) :
+  length x = ULift.down (foldl (λ ⟨n⟩ _ => ⟨n.succ⟩) ⟨0⟩ x) := by
+rw [← length_toList, toList_eq, List.length_reverse]
+let R (x : List α) (y : ULift Nat) := x.length = y.down
+apply foldl_sim (SIM := R)
+. apply Reflexive.refl
+intros a xs n; cases n with
+  | up n =>
+simp [flip]; auto
 
 end LawfulFoldable
 
 instance : Foldable List where
   foldl := List.foldl
+  toList := id
+  length := List.length
 
 instance : Foldable Array where
   foldl := Array.foldl
+  toArray := id
+  toList := Array.toList
+  length := Array.size
 
 namespace Array
 
@@ -63,6 +169,12 @@ end Array
 instance : LawfulFoldable Array where
   foldl_sim :=  by
     intros; apply Array.foldl_sim <;> auto
+  toArray_toList :=
+    by intros; simp [Array.toArray_toList, toList, toArray]
+  length_toList :=
+    by intros; simp [toList]; refl
+  foldl_toList := by
+    intros; simp [toList, foldl]
 
 namespace List
 
@@ -80,3 +192,9 @@ end List
 instance : LawfulFoldable List where
   foldl_sim :=  by
     intros; apply List.foldl_sim <;> auto
+  toArray_toList := by
+    intros; simp [toList, toArray]
+  length_toList := by
+    intros; simp [toList]; refl
+  foldl_toList := by
+    intros; simp [toList]; refl
